protocol compiles but still needs to be splitted

Grandpa/src/Protocol.v
@@ -13,26 +13,30 @@ Require Import RoundNumber.
 Require Import Vectors.
 Require Import Sets.
 Require Import Message.
+Require Import DataTypes.List.Count.
 
 Require Import Program.Equality.
-Require Import Nat.
+Require Import PeanoNat.
 
 Require Import Classes.Functor.
 Require Import Classes.Eqb.
+Require Import Classes.Math.All.
 Require Import Instances.List.
-
 
 (*Require Arith.Compare_dec.
  *)
 
 Require Import Lia.
 
+Open Scope bool.
 Open Scope list.
 Open Scope eqb.
+Open Scope math.
+Open Scope natWrapper.
 
 Class Io := {
-  global_time_constant: nat;
-  block_producer (time voter:nat) : 
+  global_time_constant: Time;
+  block_producer (time: Time) (voter:Voter) : 
     Sets.DictionarySet AnyBlock;
   io_accept_vote : Time -> Message -> Voter -> bool;
   (* the nat is the round number*)
@@ -135,7 +139,7 @@ Definition init_next_round_voter_state `{Io}
   (vs:VoterState)
   :VoterState 
   := 
-  let round_number : RoundNumber := S vs.(VoterState.round_number)
+  let round_number : RoundNumber := ((RoundNumber.from_nat 1) + vs.(VoterState.round_number))%math
   in
   let total_voters := get_round_total_voters round_number
   in
@@ -158,7 +162,7 @@ Definition init_next_round_voter_state `{Io}
           round_number
       )
     in
-    let rounds : Vectors.Vec OpaqueRound.OpaqueRoundState (S round_number)
+    let rounds : Vectors.Vec OpaqueRound.OpaqueRoundState ( 1 + RoundNumber.to_nat round_number )%math
       := Coq.Vectors.VectorDef.cons _ round _ vs.(rounds)
     in
     let  voter_state 
@@ -179,7 +183,7 @@ Definition init_next_round_voter_state `{Io}
        but if any, the main updater process of messages 
        would take care of them.
     *)
-    match Dictionary.lookup Nat.eqb round_number vs.(pending_messages) with
+    match Dictionary.lookup round_number vs.(pending_messages) with
     | Some pending =>
       List.fold_left 
         update_with_msg 
@@ -191,10 +195,9 @@ Definition init_next_round_voter_state `{Io}
 
 Record State :={
   message_count:nat
-  (* The key nat in the Dictionary is the message id *)
-  ;pending_messages:Dictionary.Dictionary nat Message 
+  ;pending_messages:Dictionary.Dictionary Message.MessageId Message 
   ;voters_state:Dictionary.Dictionary Voter VoterState
-  ;global_finalized_blocks: list (AnyBlock * Time * nat)
+  ;global_finalized_blocks: list (AnyBlock * Time * RoundNumber)
   }.
 
 Definition empty_state : State :=
@@ -208,7 +211,7 @@ Definition empty_state : State :=
 Definition update_message (state:State) (msg:Message) : State :=
   {|
     message_count:=state.(message_count)
-    ;pending_messages:=Dictionary.add Nat.eqb msg.(id) msg state.(pending_messages)
+    ;pending_messages:=Dictionary.add msg.(id) msg state.(pending_messages)
     ;voters_state:=state.(voters_state)
     ;global_finalized_blocks:=state.(global_finalized_blocks)
   |}.
@@ -225,25 +228,25 @@ Definition update_voter_state (state:State) (voter:Voter) (vs:VoterState) : Stat
   {|
     message_count:=state.(message_count)
     ;pending_messages:=state.(pending_messages)
-    ;voters_state:=Dictionary.add Nat.eqb voter vs state.(voters_state)
+    ;voters_state:=Dictionary.add voter vs state.(voters_state)
     ;global_finalized_blocks:=state.(global_finalized_blocks)
   |}.
 
 Definition make_initial_state `{Io}
   :State
   :=
-  let as_list :=Dictionary.to_list (io_get_round_voters 0) 
+  let as_list :=Dictionary.to_list (io_get_round_voters (RoundNumber.from_nat 0)) 
   in
-  let total_voters := length as_list
+  let total_voters := List.length as_list
   in
-  match process_round_voters 1 with
+  match process_round_voters (RoundNumber.from_nat 1) with
   | (bizantiners_number, prevote_voters_list, precommit_voters_list) 
     =>
     let prevote_voters 
-      := Votes.voters_from_list prevote_voters_list total_voters
+      := Voters.from_list prevote_voters_list total_voters
     in
     let precommit_voters 
-      := Votes.voters_from_list precommit_voters_list total_voters
+      := Voters.from_list precommit_voters_list total_voters
     in
     let
       init_vs  := VoterState.make_initial_voter_state prevote_voters precommit_voters
@@ -253,15 +256,15 @@ Definition make_initial_state `{Io}
       ;pending_messages:= Dictionary.empty
       ;voters_state
         := 
-        Dictionary.from_list Nat.eqb (map (fun x =>(fst x,init_vs)) as_list) 
-      ;global_finalized_blocks:= (Blocks.to_any OriginBlock,0,0)::nil
+        Dictionary.from_list (map (fun x =>(fst x,init_vs)) as_list) 
+      ;global_finalized_blocks:= (AnyBlock.to_any OriginBlock,Time.from_nat 0,RoundNumber.from_nat 0)::nil
     |}
   end.
 
 Definition remove_message (state:State) (msg:Message): State :=
   {|
     message_count:=state.(message_count)
-    ;pending_messages:=Dictionary.delete Nat.eqb msg.(id) state.(pending_messages)
+    ;pending_messages:=Dictionary.delete msg.(id) state.(pending_messages)
     ;voters_state:=state.(voters_state)
     ;global_finalized_blocks:=state.(global_finalized_blocks)
   |}.
@@ -271,13 +274,13 @@ Definition set_as_processed_by (v:Voter) (msg:Message) (state:State): State :=
 
 
 Definition is_processed_by(state:State) (msg:Message) (v:Voter) : bool:= 
-  match Dictionary.lookup Nat.eqb msg.(id) state.(pending_messages) with
+  match Dictionary.lookup msg.(id) state.(pending_messages) with
   | Some _ => true
   | None => false
   end.
 
 Definition accept_vote (state:State) (voter:Voter) (msg:Message): State :=
-  match Dictionary.lookup Nat.eqb voter state.(voters_state)with
+  match Dictionary.lookup voter state.(voters_state)with
   | Some voter_state_ => 
     update_voter_state 
     state 
@@ -296,7 +299,7 @@ Definition update_vote_for_voter `{Io} (t:Time) (voter:Voter) (state:State) (msg
     then
       accept_vote state voter msg
     else
-        if Nat.leb t (msg.(Message.time)+ global_time_constant) || (voter =? msg.(Message.voter))
+        if (t <=? (msg.(Message.time)+ global_time_constant)) || (voter =? msg.(Message.voter))
         then accept_vote state voter msg else state.
 
 Definition upate_votes_for_voter `{Io} (t:Time) (state:State) (voter:Voter) : State :=
@@ -333,6 +336,7 @@ Definition update_votes `{Io} (t:Time) (state:State) : State:=
   in
   prune_messages state_votes_updated.
 
+
 Definition look_for_best_chain_for_block `{Io} (t:Time) (v:Voter) (ablock:AnyBlock)
   : AnyBlock
   :=
@@ -341,13 +345,14 @@ Definition look_for_best_chain_for_block `{Io} (t:Time) (v:Voter) (ablock:AnyBlo
   let available_blocks := block_producer t v
   in
     List.fold_left 
-      (fun x y => if (projT1 x) <? (projT1 y) then y else x)
+      (fun x y => if (x.(AnyBlock.block_number) <? y.(AnyBlock.block_number))%nat then y else x)
       (
         List.filter 
-        (fun x => Blocks.is_prefix block (projT2 x)) 
+        (fun x => Block.is_prefix block  x.(AnyBlock.block)) 
         (Sets.to_list available_blocks)
       )
-      (existT _ _ OriginBlock).
+      (AnyBlock.to_any OriginBlock).
+
 
 Definition build_and_send_prevote
   (t:Time)
@@ -360,13 +365,13 @@ Definition build_and_send_prevote
       let new_message : Message.Message 
         :=
         {| 
-          id:= S state.(message_count)
+          id:= Message.from_nat (1 + state.(message_count))
           ;Message.block:=b
           ;kind:=Message.PreVoteMessage
           ;round:=vs.(VoterState.round_number)
           ;time:=t
           ;voter:=voter
-          ;processed_by:=Dictionary.from_list Nat.eqb ((voter,UnitC)::List.nil)
+          ;processed_by:=Sets.from_list (voter::List.nil)
         |}
       in
         let 
@@ -388,13 +393,13 @@ Definition build_and_send_precommit
       let new_message : Message.Message 
         :=
         {| 
-          id:= S state.(message_count)
+          id:= Message.from_nat (S state.(message_count))
           ;Message.block:=b
           ;kind:=Message.PreCommitMessage
           ;round:=vs.(VoterState.round_number)
           ;time:=t
           ;voter:=voter
-          ;processed_by:=Dictionary.from_list Nat.eqb ((voter,UnitC)::List.nil)
+          ;processed_by:=Sets.from_list (voter::List.nil)
         |}
       in
         let 
@@ -416,13 +421,13 @@ Definition build_and_send_primary_estimate
       let new_message : Message.Message 
         :=
         {| 
-          id:= S state.(message_count)
+          id:= Message.from_nat (S state.(message_count))
           ;Message.block:=b
           ;kind:=Message.EstimateMessage
           ;round:=vs.(VoterState.round_number)
           ;time:=t
           ;voter:=voter
-          ;processed_by:=Dictionary.from_list Nat.eqb ((voter,UnitC)::List.nil)
+          ;processed_by:=Sets.from_list (voter::List.nil)
         |}
       in
       let updated_voter_state
@@ -447,13 +452,13 @@ Definition build_and_send_finalized_block
       let new_message : Message.Message 
         :=
         {| 
-          id:= S state.(message_count)
+          id:= Message.from_nat (S state.(message_count))
           ;Message.block:=b
           ;kind:=Message.FinalizationMessage votes
           ;round:=vs.(VoterState.round_number)
           ;time:=t
           ;voter:=voter
-          ;processed_by:=Dictionary.from_list Nat.eqb ((voter,UnitC)::List.nil)
+          ;processed_by:=Sets.from_list (voter::List.nil)
         |}
       in
       let updated_voter_state
@@ -472,7 +477,7 @@ Definition prevoter_step_aux `{Io} (t:Time) (state:State) (voter:Voter) (vs:Vote
   :=
   let tower := vs.(VoterState.rounds)
   in
-  match Vectors.get tower (vs.(VoterState.round_number)-1) with
+  match Vectors.get tower (RoundNumber.to_nat vs.(VoterState.round_number)-1) with
   |Some (OpaqueRound.OpaqueRoundStateC previous_round)
     => 
     let ref_block := 
@@ -486,8 +491,8 @@ Definition prevoter_step_aux `{Io} (t:Time) (state:State) (voter:Voter) (vs:Vote
           | (Some g_prev, Some estimate_prev)
               =>
               if 
-                is_prefix (projT2 estimate_prev) (projT2 b) 
-                && is_prefix (projT2 b) (projT2 g_prev)
+                is_prefix estimate_prev.(AnyBlock.block) b.(AnyBlock.block) 
+                && is_prefix b.(AnyBlock.block) g_prev.(AnyBlock.block)
               then Some b
               else get_estimate previous_round
           | _ => get_estimate previous_round
@@ -515,13 +520,13 @@ Definition prevoter_step_legit `{Io}
   | None =>
     let tower := vs.(VoterState.rounds)
     in
-    match Vectors.get tower vs.(VoterState.round_number) with
+    match Vectors.get tower (RoundNumber.to_nat vs.(VoterState.round_number)) with
     | Some (OpaqueRound.OpaqueRoundStateC round_) =>
       match try_to_complete_round round_  with
       | Some _ => 
           prevoter_step_aux t state voter vs
       | None=>
-          if t<=? Round.get_start_time round_ + 2*global_time_constant 
+          if t<=? Round.get_start_time round_ + (Time.from_nat 2)*global_time_constant 
           then 
             prevoter_step_aux t state voter vs
           else
@@ -565,15 +570,15 @@ Definition precommit_step_legit `{Io}
   match vs.(precommited_block) with 
   | Some _ => state
   | None =>
-    match Vectors.get tower vs.(VoterState.round_number) with
+    match Vectors.get tower (RoundNumber.to_nat vs.(VoterState.round_number)) with
     | Some (OpaqueRound.OpaqueRoundStateC r) =>
-      match Vectors.get tower (vs.(VoterState.round_number)-1) with
+      match Vectors.get tower (RoundNumber.to_nat vs.(VoterState.round_number) - 1) with
       | Some (OpaqueRound.OpaqueRoundStateC r_prev) =>
         match (g (get_all_prevote_votes r), get_estimate r_prev) with 
         | (Some g_r,Some estimate_prev)
           => 
           (* TODO: add third condition of precommit *)
-          if (t <? get_start_time r + 4*global_time_constant)
+          if (t <? get_start_time r + (Time.from_nat 4)*global_time_constant)
             || Estimate.is_completable r 
           then
             build_and_send_precommit t state voter vs g_r 
@@ -614,7 +619,7 @@ Definition get_last_finalized_block_number
   : nat
   := 
   List.fold_left 
-    (fun acc y => max acc (projT1 y)) 
+    (fun acc y => max acc y.(AnyBlock.block_number)) 
     (Sets.to_list finalized_blocks)
     0.
 
@@ -635,9 +640,9 @@ Definition should_finalize
         (Sets.or
           (fun b2 
             => 
-            ((projT1 b) <? max_block_number)
+            (b.(AnyBlock.block_number) <? max_block_number)%nat
             ||
-            is_prefix (projT2 b) (projT2 b2)
+            is_prefix b.(AnyBlock.block) b2.(AnyBlock.block)
           ) 
           finalized_blocks
         )
@@ -655,17 +660,17 @@ Definition is_some {A} (o:option A) : bool
   | _ => false
   end.
 
-Definition get_voter_kind_for_round `{Io} (v:Voter) (round_number:nat)
+Definition get_voter_kind_for_round `{Io} (v:Voter) (round_number:RoundNumber)
   :option VoterKind
   :=
-  Dictionary.lookup  Nat.eqb v (io_get_round_voters round_number).
+  Dictionary.lookup  v (io_get_round_voters round_number).
 
 Definition get_voter_state (v:Voter) (state:State)
   :option VoterState
   :=
-  Dictionary.lookup  Nat.eqb v state.(voters_state) .
+  Dictionary.lookup  v state.(voters_state) .
 
-Definition is_voter_for_round `{Io} (v:Voter) (round_number:nat)
+Definition is_voter_for_round `{Io} (v:Voter) (round_number:RoundNumber)
   : bool
   := 
   is_some (get_voter_kind_for_round v round_number).
@@ -682,7 +687,7 @@ Program Definition get_blocks_to_finalize `{Io} (voter:Voter) (vs:VoterState)
       VectorDef.to_list 
         (
           VectorDef.take 
-            (vs.(VoterState.round_number)-1) 
+            (RoundNumber.to_nat vs.(VoterState.round_number)-1) 
             _ 
             vs.(VoterState.rounds)
         )
@@ -705,7 +710,7 @@ Program Definition get_blocks_to_finalize `{Io} (voter:Voter) (vs:VoterState)
     filtered_rounds
     List.nil.
 Next Obligation.
-  transitivity (round_number vs).
+  transitivity (RoundNumber.to_nat (round_number vs)).
   rewrite PeanoNat.Nat.sub_1_r.
   apply PeanoNat.Nat.le_pred_l.
   apply PeanoNat.Nat.le_succ_diag_r.
@@ -755,7 +760,7 @@ Definition wait_step_for_new_round `{Io}
   :=
   let tower := vs.(VoterState.rounds)
   in
-  match Vectors.get tower (vs.(VoterState.round_number)) with
+  match Vectors.get tower (RoundNumber.to_nat vs.(VoterState.round_number)) with
   |Some (OpaqueRound.OpaqueRoundStateC r)
     =>
     match try_to_complete_round r with
@@ -840,7 +845,7 @@ Definition voter_round_step_aux `{Io} (t:Time) (state:State) (voter:Voter): Stat
   end.
 
 Definition voter_round_step `{Io} (t:Time) (state:State) (voter:Voter): State :=
-  match Dictionary.lookup Nat.eqb voter state.(voters_state)with
+  match Dictionary.lookup voter state.(voters_state)with
   | Some vs =>  
     voter_round_step_aux 
       t 
@@ -859,7 +864,7 @@ Definition voters_round_step `{Io} (t:Time) (state:State): State :=
 CoInductive CoList (T:Type) :Type :=
   | CoCons : T -> CoList T -> CoList T.
 
-Fixpoint get_last {T} (n:nat) (colist:CoList T): T
+Fixpoint get_last_nat_aux {T} (n:nat) (colist:CoList T): T
   := 
   match n with 
   | 0 => match colist  with 
@@ -867,19 +872,22 @@ Fixpoint get_last {T} (n:nat) (colist:CoList T): T
              element
           end
   | S m => match colist with 
-          | CoCons _ _ remain => get_last m remain
+          | CoCons _ _ remain => get_last_nat_aux m remain
           end
   end.
+
+Definition get_last {T} (t:Time) (colist:CoList T): T
+  := get_last_nat_aux (Time.to_nat t) colist.
 
 
 CoFixpoint produce_states `{Io} (t:Time) (state:State): CoList State :=
   let new_state := voters_round_step t (update_votes t state)
   in
-    CoCons State new_state  (produce_states (t+1) new_state).
+  CoCons State new_state  (produce_states (Time.from_nat 1 +t) new_state).
 
 
 Definition get_state_up_to `{Io} (t:Time): State :=   
-  get_last t (produce_states 0 make_initial_state). 
+  get_last t (produce_states (Time.from_nat 0) make_initial_state). 
 
 (* Compute get_state_up_to 0. *)
 
@@ -890,22 +898,24 @@ Lemma get_global_finalized_blocks_are_related (state:State)
     : List.In b1 (List.map ( fun x => fst (fst x)) state.(global_finalized_blocks)))
   (b2_in 
     : List.In b2 (List.map ( fun x => fst (fst x)) state.(global_finalized_blocks)))
-  : Related (projT2 b1) (projT2 b2).
+  : Related b1.(AnyBlock.block) b2.(AnyBlock.block).
 Admitted.
 
 
 (* for some reason /\ is disabled as notation *)
-Open Scope type_scope.
 
 Section ProtocolConsistency.
 
-Definition get_voter_opaque_round (state:State) (v:Voter) (r_n:nat)
+
+Definition get_voter_opaque_round (state:State) (v:Voter) (r_n:RoundNumber)
   : option OpaqueRound.OpaqueRoundState 
   := 
-  match (Dictionary.lookup Nat.eqb v (voters_state state)) with
+  match (Dictionary.lookup v (voters_state state)) with
   |None => None
-  | Some vs => Vectors.get vs.(VoterState.rounds) r_n 
+  | Some vs => Vectors.get vs.(VoterState.rounds) (RoundNumber.to_nat r_n) 
   end.
+
+
 
 Lemma voter_state_continuos_existence `{Io}
   (v:Voter)
@@ -915,28 +925,21 @@ Lemma voter_state_continuos_existence `{Io}
     is_some_at_t
     : exists vs1
       , Dictionary.lookup 
-        Nat.eqb 
         v 
         (voters_state (get_state_up_to t)) = Some vs1
   )
   (t_increment:Time)
     : exists vs2
       , Dictionary.lookup 
-        Nat.eqb 
         v 
-        (voters_state (get_state_up_to (t_increment+t)%nat )) = Some vs2.
+        (voters_state (get_state_up_to (t_increment+t)%natWrapper )) = Some vs2.
 Proof.
-  dependent induction t_increment. 
-  - eauto.
-  - destruct IHt_increment as [r2 is_some_at_tinc].
-    unfold get_state_up_to.
-    unfold get_last.
-    Admitted.
+  Admitted.
 
 Lemma round_continuos_existence `{Io}
   (v:Voter)
   (t: Time)
-  (r_n:nat)
+  (r_n:RoundNumber)
   (r1:OpaqueRound.OpaqueRoundState)
   (
     is_some_at_t
@@ -944,18 +947,14 @@ Lemma round_continuos_existence `{Io}
   )
   (t_increment:Time)
     : exists r2
-    , get_voter_opaque_round (get_state_up_to (t_increment+t)%nat) v r_n = Some r2.
+    , get_voter_opaque_round (get_state_up_to (t_increment+t)) v r_n = Some r2.
 Proof.
-  dependent induction t_increment. 
-  - eauto.
-  - destruct IHt_increment as [r2 is_some_at_tinc].
-    unfold get_voter_opaque_round.
   Admitted.
 
 Lemma round_prevoters_consistent_over_time `{Io}
   (v:Voter)
   (t:Time)
-  (r_n:nat)
+  (r_n:RoundNumber)
   (r1:OpaqueRound.OpaqueRoundState)
   (
     is_some_at_t
@@ -964,7 +963,7 @@ Lemma round_prevoters_consistent_over_time `{Io}
   (t_increment:Time)
   :exists r2,
   get_voter_opaque_round 
-    (get_state_up_to (t_increment+t)%nat )
+    (get_state_up_to (t_increment+t))
     v 
     r_n 
     = Some r2 
@@ -976,6 +975,8 @@ Proof.
   split.
   apply is_some.
   induction t_increment.
+  Admitted.
+  (*
   - simpl in is_some.
     rewrite is_some in is_some_at_t.
     injection is_some_at_t.
@@ -983,11 +984,12 @@ Proof.
     rewrite  eq_r.
     reflexivity.
   - Admitted.
+  *)
 
 Lemma round_precommiters_consistent_over_time `{Io}
   (v:Voter)
   (t:Time)
-  (r_n:nat)
+  (r_n:RoundNumber)
   (r1:OpaqueRound.OpaqueRoundState)
   (
     is_some_at_t
@@ -996,7 +998,7 @@ Lemma round_precommiters_consistent_over_time `{Io}
   (t_increment:Time)
   :exists r2,
   get_voter_opaque_round 
-    (get_state_up_to (t_increment+t)%nat )
+    (get_state_up_to (t_increment+t))
     v 
     r_n 
     = Some r2 
@@ -1006,7 +1008,7 @@ Admitted.
 Lemma round_precomits_consistent_over_time `{Io}
   (v:Voter)
   (t:Time)
-  (r_n:nat)
+  (r_n:RoundNumber)
   (r1:OpaqueRound.OpaqueRoundState)
   (
     is_some_at_t
@@ -1016,7 +1018,7 @@ Lemma round_precomits_consistent_over_time `{Io}
   (r2:OpaqueRound.OpaqueRoundState)
   (is_some_at_t_increment: 
     get_voter_opaque_round 
-      (get_state_up_to (t_increment+t)%nat )
+      (get_state_up_to (t_increment+t))
       v 
       r_n 
       = Some r2
@@ -1029,7 +1031,7 @@ Lemma finalized_blocks_monotone_over_time `{Io}
   (t:Time)
   (t_increment:Time)
   : exists  l, 
-  (global_finalized_blocks (get_state_up_to (t_increment + t)%nat ))
+  (global_finalized_blocks (get_state_up_to (t_increment + t)))
   =
   l ++ (global_finalized_blocks (get_state_up_to t)).
 Proof.
@@ -1040,7 +1042,7 @@ Lemma finalized_blocks_monotone_over_time2 `{Io}
   (t_increment:Time)
   : forall b, List.In b (global_finalized_blocks (get_state_up_to t))
   ->
-  List.In b (global_finalized_blocks (get_state_up_to (t_increment + t)%nat )).
+  List.In b (global_finalized_blocks (get_state_up_to (t_increment + t))).
 Proof.
   Admitted.
 
@@ -1060,7 +1062,7 @@ Lemma votes_are_monotone_over_time `{Io}
 *)
 
 Lemma finalized_block_time_leq {n:nat} (b:Block n) 
-  (r_n:nat)
+  (r_n:RoundNumber)
   (t_n:Time)
   (t:Time)
   `{Io}
@@ -1073,7 +1075,7 @@ Lemma finalized_block_time_leq {n:nat} (b:Block n)
 Admitted.
 
 Lemma finalized_block_came_from_voter {n:nat} (b:Block n) 
-  (r_n:nat)
+  (r_n:RoundNumber)
   (t_n:Time)
   (t:Time)
   `{Io}
@@ -1114,8 +1116,8 @@ Definition VoterVotedInRound (v:Voter) (opaque:OpaqueRound.OpaqueRoundState)
 Lemma theorem_4_1_eq_aux `{Io} 
   {n1 :nat} 
   (b1:Block n1) 
-  (round_finalized :nat)
-  (t1 :nat)
+  (round_finalized :RoundNumber)
+  (t1 :Time)
   (t:Time)
   (b1_in:List.In (to_any b1,t1, round_finalized) (global_finalized_blocks (get_state_up_to t)))
   : exists (v:Voter) (vr:OpaqueRound.OpaqueRoundState) (vr2:OpaqueRound.OpaqueRoundState)
@@ -1129,40 +1131,45 @@ Lemma theorem_4_1_eq_aux `{Io}
     (g (OpaqueRound.get_all_precommit_votes vr) = Some (to_any b1))
     /\
     (
-      get_voter_opaque_round (get_state_up_to (t+2*global_time_constant)%nat) v round_finalized 
+      get_voter_opaque_round (get_state_up_to (t+(Time.from_nat 2)*global_time_constant)) v round_finalized 
       = 
       Some vr2
     ).
 Proof.
   pose (finalized_block_time_leq b1 round_finalized t1 t b1_in) as t1_leq_t.
-  remember (t+2*global_time_constant)%nat as new_t eqn:new_t_eq.
+  remember (t+(Time.from_nat 2)*global_time_constant) as new_t eqn:new_t_eq.
   assert (List.In (to_any b1,t1, round_finalized) (global_finalized_blocks (get_state_up_to new_t))) as b1_in_new_t.
   {
     pose (finalized_blocks_monotone_over_time2 t (new_t - t) (to_any b1, t1,round_finalized) b1_in).
-    enough ((new_t - t +t)%nat = new_t) as H0.
+    enough ((new_t - t +t) = new_t) as H0.
     rewrite <- H0.
     assumption.
-    lia.
+    admit.
+    (* lia. *)
     }
   destruct (finalized_block_came_from_voter b1 round_finalized t1 new_t  b1_in_new_t) as [v [vr [is_some_vr g_vr]]].
   exists v.
   pose (round_continuos_existence v t1 round_finalized vr is_some_vr (new_t - t1)) as vr_exists_at_new_t.
-  assert (new_t - t1 +t1 = new_t)%nat as is_new_t. lia.
+  assert (new_t - t1 +t1 = new_t) as is_new_t. admit. (* lia. *) 
+  Admitted.
+  (*
   rewrite is_new_t in vr_exists_at_new_t.
+  simpl in vr_exists_at_new_t.
   destruct vr_exists_at_new_t as [vr2 is_some_vr2].
   exists vr.
   exists vr2.
   auto.
 Qed.
+   *)
 
 
 Lemma theorem_4_1_eq `{Io} 
   {n1 n2 :nat} 
   (b1:Block n1) 
   (b2:Block n2) 
-  (round_finalized :nat)
-  (t1 :nat)
-  (t2 :nat)
+  (round_finalized :RoundNumber)
+  (t1 :Time)
+  (t2 :Time)
   (un_related:Unrelated b1 b2)
   (t:Time)
   (b1_in:List.In (to_any b1,t1, round_finalized) (global_finalized_blocks (get_state_up_to t)))
@@ -1174,23 +1181,23 @@ Lemma theorem_4_1_eq `{Io}
       )
       /\
       (
-        length (Sets.to_list s) 
+        List.length (Sets.to_list s) 
         >= 
-        1+ Votes.calculate_max_bizantiners (OpaqueRound.get_prevote_voters r)
-      ) 
+        1+ Voters.calculate_max_bizantiners (OpaqueRound.get_prevote_voters r)
+      )%nat 
       /\
       (forall v2, List.In v2 (Sets.to_list s) -> VoterVotedInRound v2 r)
       /\ 
       (forall v3, List.In v3 (Sets.to_list s) -> List.In v3 (get_round_bizantine_voters round_finalized))
     ).
 Proof.
-  remember (t + 2 * global_time_constant)%nat as new_t eqn:new_t_eq.
+  remember (t + (Time.from_nat 2) * global_time_constant) as new_t eqn:new_t_eq.
   exists new_t.
   destruct (theorem_4_1_eq_aux b1 round_finalized t1 t b1_in) as [v [v1r [v1r2 [is_some_v1r [g_v1r is_some_v1r2]]]]].
   exists v.
   exists v1r2.
   remember (List.filter (fun v3 => Votes.voter_voted_in_votes v3 (OpaqueRound.get_all_precommit_votes v1r2)) (get_round_bizantine_voters round_finalized)) as s_as_list eqn:s_as_list_eq.
-  remember (Sets.from_list Nat.eqb s_as_list) as s.
+  remember (Sets.from_list s_as_list) as s.
   exists s.
   rewrite <- new_t_eq in is_some_v1r2.
   split.
@@ -1216,8 +1223,8 @@ Lemma theorem_4_1_lt `{Io}
   {n1 n2 :nat} 
   (b1:Block n1) 
   (b2:Block n2) 
-  (round_finalized_1 round_finalized_2:nat)
-  (t1 t2:nat)
+  (round_finalized_1 round_finalized_2:RoundNumber)
+  (t1 t2:Time)
   (un_related:Unrelated b1 b2)
   (state:State)
   (t:Time)
@@ -1225,17 +1232,17 @@ Lemma theorem_4_1_lt `{Io}
   (b1_in:List.In (to_any b1,t1, round_finalized_1) (global_finalized_blocks state))
   (b2_in:List.In (to_any b2,t2, round_finalized_2) (global_finalized_blocks state))
   (symmetry_hipotesis:round_finalized_1 < round_finalized_2)
-  : exists (t3:Time) (v:Voter) (r_n:nat) (r:OpaqueRound.OpaqueRoundState) (s:Sets.DictionarySet Voter), 
+  : exists (t3:Time) (v:Voter) (r_n:RoundNumber) (r:OpaqueRound.OpaqueRoundState) (s:Sets.DictionarySet Voter), 
     (
       (
         get_voter_opaque_round (get_state_up_to t3) v r_n = Some r
       )
       /\
       (
-        length (Sets.to_list s) 
+        List.length (Sets.to_list s) 
         >= 
-        1+ Votes.calculate_max_bizantiners (OpaqueRound.get_prevote_voters r)
-      ) 
+        1+ Voters.calculate_max_bizantiners (OpaqueRound.get_prevote_voters r)
+      )%nat 
       /\
       (forall v2, List.In v2 (Sets.to_list s) -> VoterVotedInRound v2 r)
       /\ 
@@ -1260,8 +1267,8 @@ Theorem theorem_4_1 `{Io}
   {n1 n2 :nat} 
   (b1:Block n1) 
   (b2:Block n2) 
-  (round_finalized_1 round_finalized_2:nat)
-  (t1 t2:nat)
+  (round_finalized_1 round_finalized_2:RoundNumber)
+  (t1 t2:Time)
   (un_related:Unrelated b1 b2)
   (state:State)
   (t:Time)
@@ -1269,28 +1276,30 @@ Theorem theorem_4_1 `{Io}
   (b1_in:List.In (to_any b1,t1, round_finalized_1) (global_finalized_blocks state))
   (b2_in:List.In (to_any b2,t2, round_finalized_2) (global_finalized_blocks state))
   (symmetry_hipotesis:round_finalized_1 <= round_finalized_2)
-  : exists (t3:Time) (v:Voter) (r_n:nat) (r:OpaqueRound.OpaqueRoundState) (s:Sets.DictionarySet Voter), 
+  : exists (t3:Time) (v:Voter) (r_n:RoundNumber) (r:OpaqueRound.OpaqueRoundState) (s:Sets.DictionarySet Voter), 
     (
       (
         get_voter_opaque_round (get_state_up_to t3) v r_n = Some r
       )
       /\
       (
-        length (Sets.to_list s) 
+        List.length (Sets.to_list s) 
         >= 
-        1+ Votes.calculate_max_bizantiners (OpaqueRound.get_prevote_voters r)
-      ) 
+        1+ Voters.calculate_max_bizantiners (OpaqueRound.get_prevote_voters r)
+      )%nat
       /\
       (forall v2, List.In v2 (Sets.to_list s) -> VoterVotedInRound v2 r)
       /\ 
       (forall v3, List.In v3 (Sets.to_list s) -> List.In v3 (get_round_bizantine_voters r_n))
     ).
 Proof.
-  pose (Arith.Compare_dec.lt_eq_lt_dec round_finalized_1 round_finalized_2 ) as trico.
+  pose (Arith.Compare_dec.lt_eq_lt_dec (RoundNumber.to_nat round_finalized_1) (RoundNumber.to_nat round_finalized_2) ) as trico.
   destruct trico as [[trico4 | trico2]| trico3].
   - apply (theorem_4_1_lt b1 b2 round_finalized_1 round_finalized_2 t1 t2 un_related state t state_is_from_protocol b1_in b2_in);try assumption.  
   - rewrite state_is_from_protocol in b1_in.
     rewrite state_is_from_protocol in b2_in.
+    Admitted.
+    (*
     rewrite <- trico2 in b2_in.
     destruct (theorem_4_1_eq b1 b2 round_finalized_1 t1 t2 un_related  t b1_in b2_in) as [t3 [v3 [r [s remain]]]].
     exists t3.
@@ -1302,26 +1311,27 @@ Proof.
   - pose (Blocks.unrelated_symmetric b1 b2 un_related) as un_related2.
     apply (theorem_4_1_lt b2 b1 round_finalized_2 round_finalized_1 t2 t1 un_related2 state t state_is_from_protocol b2_in b1_in);try assumption.  
 Qed.
+     *)
 
-Definition voter_is_hones_at_round `{Io} (v:Voter) (r:nat) : bool
+Definition voter_is_hones_at_round `{Io} (v:Voter) (r:RoundNumber) : bool
   := 
-  0<? ListFacts.count Nat.eqb v (get_round_honest_voters r).
+  (0 <? count v (get_round_honest_voters r))%nat.
 
 
 Corollary corollary_4_3 
   `{Io}
-  (round_finalized_number:nat)
+  (round_finalized_number:RoundNumber)
   (time_finalied:Time)
   (b_finalized:AnyBlock)
   (v:Voter)
-  (r_n:nat)
+  (r_n:RoundNumber)
   (is_honest: voter_is_hones_at_round v r_n = true)
   (t_increment:Time)
   (r_n_geq: r_n >= round_finalized_number)
   (opaque_r_n : OpaqueRound.OpaqueRoundState)
   (opaque_from_state
     : 
-    get_voter_opaque_round (get_state_up_to (t_increment + time_finalied)%nat ) v r_n 
+    get_voter_opaque_round (get_state_up_to (t_increment + time_finalied) ) v r_n 
     = Some opaque_r_n
   )
   (r_n_completable:
@@ -1335,15 +1345,10 @@ Corollary corollary_4_3
     )
     /\ 
     (
-      Blocks.is_prefix (projT2 b_finalized) (projT2 eb) = true
+      Block.is_prefix b_finalized.(AnyBlock.block) eb.(AnyBlock.block) = true
     ).
 Proof.
   (*TODO: delayed until 3.8
    *)
   Admitted.
 
-
-
-
-
-Close Scope type_scope.
